Test/dafny1/PriorityQueue.dfy
@@ -2,45 +2,42 @@
 // RUN: %diff "%s.expect" "%t"
 
 class PriorityQueue {
-  var N: int;  // capacity
-  var n: int;  // current size
-  ghost var Repr: set<object>;  // set of objects that make up the representation of a PriorityQueue
+  var N: nat  // capacity
+  var n: nat  // current size
+  ghost var Repr: set<object>  // set of objects that make up the representation of a PriorityQueue
 
-  var a: array<int>;  // private implementation of PriorityQueue
+  var a: array<int>  // private implementation of PriorityQueue
 
   predicate Valid()
-    reads this, Repr;
+    reads this, Repr
   {
     MostlyValid() &&
-    (forall j :: 2 <= j && j <= n ==> a[j/2] <= a[j])
+    forall j :: 2 <= j <= n ==> a[j/2] <= a[j]
   }
 
   predicate MostlyValid()
-    reads this, Repr;
+    reads this, Repr
   {
     this in Repr && a in Repr &&
     a.Length == N+1 &&
-    0 <= n && n <= N
+    0 <= n <= N
   }
 
-  method Init(capacity: int)
-    requires 0 <= capacity;
-    modifies this;
-    ensures Valid() && fresh(Repr - {this});
-    ensures N == capacity;
+  constructor Init(capacity: nat)
+    ensures Valid() && fresh(Repr)
+    ensures N == capacity
   {
     N := capacity;
-    a := new int[N+1];
+    a := new int[capacity + 1];
     n := 0;
-    Repr := {this};
-    Repr := Repr + {a};
+    Repr := {this, a};
   }
 
   method Insert(x: int)
-    requires Valid() && n < N;
-    modifies this, a;
-    ensures Valid() && fresh(Repr - old(Repr));
-    ensures n == old(n) + 1 && N == old(N);
+    requires Valid() && n < N
+    modifies Repr
+    ensures Valid() && fresh(Repr - old(Repr))
+    ensures n == old(n) + 1 && N == old(N)
   {
     n := n + 1;
     a[n] := x;
@@ -48,21 +45,21 @@ class PriorityQueue {
   }
 
   method SiftUp(k: int)
-    requires 1 <= k && k <= n;
-    requires MostlyValid();
-    requires (forall j :: 2 <= j && j <= n && j != k ==> a[j/2] <= a[j]);
-    requires (forall j {:nowarn} :: 1 <= j && j <= n ==> j/2 != k);  // k is a leaf
-    modifies a;
-    ensures Valid();
+    requires 1 <= k <= n
+    requires MostlyValid()
+    requires forall j :: 2 <= j <= n && j != k ==> a[j/2] <= a[j]
+    requires forall j :: 1 <= j <= n ==> j/2 != k  // k is a leaf
+    modifies a
+    ensures Valid()
   {
     var i := k;
     assert MostlyValid();
-    while (1 < i)
-      invariant i <= k && MostlyValid();
-      invariant (forall j :: 2 <= j && j <= n && j != i ==> a[j/2] <= a[j]);
-      invariant (forall j :: 1 <= j/2/2 && j/2 == i && j <= n ==> a[j/2/2] <= a[j]);
+    while 1 < i
+      invariant i <= k && MostlyValid()
+      invariant forall j :: 2 <= j <= n && j != i ==> a[j/2] <= a[j]
+      invariant forall j :: 1 <= j/2/2 && j/2 == i && j <= n ==> a[j/2/2] <= a[j]
     {
-      if (a[i/2] <= a[i]) {
+      if a[i/2] <= a[i] {
         return;
       }
       a[i/2], a[i] := a[i], a[i/2];
@@ -71,10 +68,10 @@ class PriorityQueue {
   }
 
   method RemoveMin() returns (x: int)
-    requires Valid() && 1 <= n;
-    modifies this, a;
-    ensures Valid() && fresh(Repr - old(Repr));
-    ensures n == old(n) - 1;
+    requires Valid() && 1 <= n
+    modifies Repr
+    ensures Valid() && fresh(Repr - old(Repr))
+    ensures n == old(n) - 1
   {
     x := a[1];
     a[1] := a[n];
@@ -83,28 +80,28 @@ class PriorityQueue {
   }
 
   method SiftDown(k: int)
-    requires 1 <= k;
-    requires MostlyValid();
-    requires (forall j  {:nowarn } {:matchinglooprewrite false} :: 2 <= j && j <= n && j/2 != k ==> a[j/2] <= a[j]);
-    requires (forall j  {:nowarn } {:matchinglooprewrite false} :: 2 <= j && j <= n && 1 <= j/2/2 && j/2/2 != k ==> a[j/2/2] <= a[j]);
+    requires 1 <= k
+    requires MostlyValid()
+    requires forall j :: 2 <= j <= n && j/2 != k ==> a[j/2] <= a[j]
+    requires forall j :: 2 <= j <= n && 1 <= j/2/2 != k ==> a[j/2/2] <= a[j]
     // Alternatively, the line above can be expressed as:
-    //     requires (forall j :: 1 <= k/2 && j/2 == k && j <= n ==> a[j/2/2] <= a[j]);
-    modifies a;
-    ensures Valid();
+    //     requires forall j :: 1 <= k/2 && j/2 == k && j <= n ==> a[j/2/2] <= a[j]
+    modifies a
+    ensures Valid()
   {
     var i := k;
-    while (2*i <= n)  // while i is not a leaf
-      invariant 1 <= i && MostlyValid();
-      invariant (forall j :: 2 <= j && j <= n && j/2 != i ==> a[j/2] <= a[j]);
-      invariant (forall j :: 2 <= j && j <= n && 1 <= j/2/2 && j/2/2 != i ==> a[j/2/2] <= a[j]);
+    while 2*i <= n  // while i is not a leaf
+      invariant 1 <= i && MostlyValid()
+      invariant forall j :: 2 <= j <= n && j/2 != i ==> a[j/2] <= a[j]
+      invariant forall j :: 2 <= j <= n && 1 <= j/2/2 != i ==> a[j/2/2] <= a[j]
     {
       var smallestChild;
-      if (2*i + 1 <= n && a[2*i + 1] < a[2*i]) {
+      if 2*i + 1 <= n && a[2*i + 1] < a[2*i] {
         smallestChild := 2*i + 1;
       } else {
         smallestChild := 2*i;
       }
-      if (a[i] <= a[smallestChild]) {
+      if a[i] <= a[smallestChild] {
         return;
       }
       a[smallestChild], a[i] := a[i], a[smallestChild];
@@ -117,45 +114,42 @@ class PriorityQueue {
 // ---------- Alternative specifications ----------
 
 class PriorityQueue_Alternative {
-  var N: int;  // capacity
-  var n: int;  // current size
-  ghost var Repr: set<object>;  // set of objects that make up the representation of a PriorityQueue
+  var N: nat  // capacity
+  var n: nat  // current size
+  ghost var Repr: set<object>  // set of objects that make up the representation of a PriorityQueue
 
-  var a: array<int>;  // private implementation of PriorityQueue
+  var a: array<int>  // private implementation of PriorityQueue
 
   predicate Valid()
-    reads this, Repr;
+    reads this, Repr
   {
     MostlyValid() &&
-    (forall j :: 2 <= j && j <= n ==> a[j/2] <= a[j])
+    forall j :: 2 <= j <= n ==> a[j/2] <= a[j]
   }
 
   predicate MostlyValid()
-    reads this, Repr;
+    reads this, Repr
   {
     this in Repr && a in Repr &&
     a.Length == N+1 &&
     0 <= n && n <= N
   }
 
-  method Init(capacity: int)
-    requires 0 <= capacity;
-    modifies this;
-    ensures Valid() && fresh(Repr - {this});
-    ensures N == capacity;
+  constructor Init(capacity: nat)
+    ensures Valid() && fresh(Repr)
+    ensures N == capacity
   {
     N := capacity;
-    a := new int[N+1];
+    a := new int[capacity + 1];
     n := 0;
-    Repr := {this};
-    Repr := Repr + {a};
+    Repr := {this, a};
   }
 
   method Insert(x: int)
-    requires Valid() && n < N;
-    modifies this, a;
-    ensures Valid() && fresh(Repr - old(Repr));
-    ensures n == old(n) + 1 && N == old(N);
+    requires Valid() && n < N
+    modifies Repr
+    ensures Valid() && fresh(Repr - old(Repr))
+    ensures n == old(n) + 1 && N == old(N)
   {
     n := n + 1;
     a[n] := x;
@@ -163,19 +157,19 @@ class PriorityQueue_Alternative {
   }
 
   method SiftUp()
-    requires MostlyValid();
-    requires (forall j :: 2 <= j && j <= n && j != n ==> a[j/2] <= a[j]);
-    modifies a;
-    ensures Valid();
+    requires MostlyValid()
+    requires forall j :: 2 <= j <= n && j != n ==> a[j/2] <= a[j]
+    modifies a
+    ensures Valid()
   {
     var i := n;
     assert MostlyValid();
-    while (1 < i)
-      invariant i <= n && MostlyValid();
-      invariant (forall j :: 2 <= j && j <= n && j != i ==> a[j/2] <= a[j]);
-      invariant (forall j :: 1 <= j/2/2 && j/2 == i && j <= n ==> a[j/2/2] <= a[j]);
+    while 1 < i
+      invariant i <= n && MostlyValid()
+      invariant forall j :: 2 <= j <= n && j != i ==> a[j/2] <= a[j]
+      invariant forall j :: 1 <= j/2/2 && j/2 == i && j <= n ==> a[j/2/2] <= a[j]
     {
-      if (a[i/2] <= a[i]) {
+      if a[i/2] <= a[i] {
         return;
       }
       a[i/2], a[i] := a[i], a[i/2];
@@ -184,10 +178,10 @@ class PriorityQueue_Alternative {
   }
 
   method RemoveMin() returns (x: int)
-    requires Valid() && 1 <= n;
-    modifies this, a;
-    ensures Valid() && fresh(Repr - old(Repr));
-    ensures n == old(n) - 1;
+    requires Valid() && 1 <= n
+    modifies Repr
+    ensures Valid() && fresh(Repr - old(Repr))
+    ensures n == old(n) - 1
   {
     x := a[1];
     a[1] := a[n];
@@ -196,24 +190,24 @@ class PriorityQueue_Alternative {
   }
 
   method SiftDown()
-    requires MostlyValid();
-    requires (forall j :: 4 <= j && j <= n ==> a[j/2] <= a[j]);
-    modifies a;
-    ensures Valid();
+    requires MostlyValid()
+    requires forall j :: 4 <= j <= n ==> a[j/2] <= a[j]
+    modifies a
+    ensures Valid()
   {
     var i := 1;
-    while (2*i <= n)  // while i is not a leaf
-      invariant 1 <= i && MostlyValid();
-      invariant (forall j :: 2 <= j && j <= n && j/2 != i ==> a[j/2] <= a[j]);
-      invariant (forall j :: 1 <= j/2/2 && j/2 == i && j <= n ==> a[j/2/2] <= a[j]);
+    while 2*i <= n  // while i is not a leaf
+      invariant 1 <= i && MostlyValid()
+      invariant forall j :: 2 <= j <= n && j/2 != i ==> a[j/2] <= a[j]
+      invariant forall j :: 1 <= j/2/2 && j/2 == i && j <= n ==> a[j/2/2] <= a[j]
     {
       var smallestChild;
-      if (2*i + 1 <= n && a[2*i + 1] < a[2*i]) {
+      if 2*i + 1 <= n && a[2*i + 1] < a[2*i] {
         smallestChild := 2*i + 1;
       } else {
         smallestChild := 2*i;
       }
-      if (a[i] <= a[smallestChild]) {
+      if a[i] <= a[smallestChild] {
         return;
       }
       a[smallestChild], a[i] := a[i], a[smallestChild];
